@prefix formats: <http://www.w3.org/ns/formats/> .

:identifiedBy
  a owl:ObjectProperty ;
  rdfs:domain rdfs:Resource ;
  schema:domainIncludes owl:NamedIndividual ;
  schema:rangeIncludes :URI ;
  dcterms:description "Specifies the identifier for a resource."@en ;
  skos:narrowMatch wdt:P2699 , schema:url .

:IANARef
  a owl:ObjectProperty ;
  rdfs:range foaf:Agent ;
  rdfs:subPropertyOf rdfs:seeAlso ;
  dcterms:description "Identifies an IANA-affiliated resource available as a reference for this entity."@en .

# URI

:URIReference
  dcterms:description "A class of URI references, either as absolute URIs or relative references. This includes IRIs."@en ;
  owl:equivalentClass [
    a owl:Class ;
    owl:unionOf ( :URI :RelativeURI )
  ] .

:URI
  rdfs:subClassOf :URIReference ;
  dcterms:description "An absolute URI or IRI."@en ;
  owl:disjointWith :RelativeURI ;
  foaf:page rfc:3986 ;
  skos:exactMatch wd:Q61694 , dbr:Uniform_Resource_Identifier .

:RelativeURI
  rdfs:subClassOf :URIReference ;
  dcterms:description "A relative URI reference which can be combined with a URI."@en ;
  foaf:page rfc:1808 ;
  owl:disjointWith :URI .

:FragmentURI
  rdfs:subClassOf :URIReference ;
  dcterms:description "A URI with a fragment identifies a portion of a resource defined by the URI reference stripped of the fragment."@en .

:URI-WellKnown
  rdfs:subClassOf :URI ;
  dcterms:description "A well-known URI is one using the HTTP or HTTPS scheme with path starting on '/.well-known/'."@en ;
  foaf:page rfc:8615 ;
  skos:exactMatch wd:Q109621265 , dbr:Well-known_URI .

:URN
  rdfs:subClassOf :URI ;
  dcterms:description "A URI using the URN scheme."@en ;
  foaf:page rfc:8141 ;
  skos:exactMatch wd:Q76497 , dbr:Uniform_Resource_Name .

:URL
  rdfs:subClassOf :URI ;
  foaf:page rfc:1738 ;
  skos:exactMatch wd:Q42253 , dbr:URL .

:PURL
  rdfs:subClassOf :URL ;
  dcterms:description "A persistent URL points to a redirect to the real resource, which can be changed if the target website is no longer available."@en ;
  skos:exactMatch wd:Q195305 , dbr:Persistent_uniform_resource_locator .

:PURL-Domain
  rdfs:subClassOf :PURL ;
  dcterms:description "A PURL domain is maintained by a single entity and defines redirects for various URLs under it."@en .


:URIDatatype-IRI
  rdfs:subClassOf xsd:anyURI ;
  dcterms:description "The identifier of an IRI."@en .

:URIDatatype-ASCII
  rdfs:subClassOf xsd:anyURI ;
  dcterms:description "The identifier of a URI, with percent-encoded non-ASCII characters."@en .


:scheme
  a owl:ObjectProperty ;
  schema:domainIncludes :URI ;
  rdfs:range :URIScheme ;
  dcterms:description "Specifies the URI scheme used by an identifier."@en ;
  skos:closeMatch wdt:P4742 .

:user
  a owl:DatatypeProperty ;
  schema:domainIncludes :URIReference ;
  rdfs:range xsd:string ;
  dcterms:description "Specifies the username stored in an identifier."@en .

:pass
  a owl:DatatypeProperty ;
  schema:domainIncludes :URIReference ;
  rdfs:range xsd:string ;
  dcterms:description "Specifies the password stored in an identifier."@en .

:account
  a owl:ObjectProperty ;
  schema:domainIncludes :URIReference ;
  rdfs:range foaf:OnlineAccount ;
  dcterms:description "Specifies the account referred to by an identifier."@en .

:host
  a owl:ObjectProperty ;
  schema:domainIncludes :URIReference ;
  rdfs:range :Host ;
  dcterms:description "Specifies the hostname referred to by an identifier."@en .

:port
  a owl:ObjectProperty ;
  schema:domainIncludes :URIReference ;
  rdfs:range :Port ;
  dcterms:description "Specifies a port referred to by an identifier. The port may also be implied by a URI scheme."@en ;
  skos:closeMatch dbp:ports , wdt:P1641 .

:noPortSpecified
  a :Port ;
  dcterms:description "Indicates that the port is not explicitly stated."@en ;
  skos:closeMatch <port/0> .

:path
  a owl:DatatypeProperty ;
  schema:domainIncludes :URIReference ;
  rdfs:range rdfs:Literal ;
  dcterms:description "Specifies the path stored by an identifier."@en .

:filename
  a owl:DatatypeProperty ;
  schema:domainIncludes :URIReference ;
  rdfs:range xsd:string ;
  dcterms:description "Specifies the file name as part of the path stored by an identifier."@en .

:suffix
  a owl:ObjectProperty ;
  schema:domainIncludes :URIReference ;
  rdfs:range :Suffix ;
  dcterms:description "Specifies the file suffix indicating the type of the file refererred to by an identifier."@en .

:query
  a owl:ObjectProperty ;
  schema:domainIncludes :URIReference ;
  rdfs:range :URIPart ;
  dcterms:description "Specifies the query part of an identifier."@en .

:fragment
  a owl:ObjectProperty ;
  schema:domainIncludes :FragmentURI ;
  rdfs:range :URIPart ;
  dcterms:description "Specifies the fragment part of an identifier."@en .

:fragmentOf
  a owl:ObjectProperty ;
  schema:domainIncludes :FragmentURI ;
  schema:rangeIncludes :URIReference ;
  dcterms:description "Specifies the base identifier which the subject one is a fragment of."@en .

:urnNamespace
  a owl:ObjectProperty ;
  schema:domainIncludes :URN ;
  rdfs:range :URNNamespace ;
  dcterms:description "Specifies the URN namespace used by an identifier."@en .

:wellknownSuffix
  a owl:ObjectProperty ;
  schema:domainIncludes :URI-WellKnown ;
  rdfs:range :WellKnownURISuffix ;
  dcterms:description "Specifies the well-known URI suffix used by an identifier."@en .

:purlDomain
  schema:domainIncludes :URIReference ;
  schema:rangeIncludes :URIReference ;
  dcterms:description "Specifies the PURL domain used by an identifier."@en .


# URI Scheme

:URIScheme
  dcterms:description "A URI scheme defines the structure and interpretation of URIs using it."@en ;
  foaf:page <https://www.iana.org/assignments/uri-schemes/uri-schemes.xhtml> ;
  skos:exactMatch wd:Q37071 .


:URISchemeDatatype
  dcterms:description "The identifier of a URI scheme."@en .

# Host

:Host
  dcterms:description "The class of all URI hostnames, either domains or IP addresses."@en ;
  skos:exactMatch wd:Q1073408 .

:HostDatatype
  dcterms:description "The identifier of a host, using international characters."@en .

:HostDatatype-Encoded
  dcterms:description "The identifier of a host, using ASCII only."@en .

:Domain
  rdfs:subClassOf :Host ;
  dcterms:description "A class of domain names that serve as identification of internet domains."@en ;
  owl:disjointWith :IP ;
  skos:exactMatch wd:Q32635 , dbr:Domain_name .

:Domain-Special
  rdfs:subClassOf :Domain ;
  dcterms:description "A domain name that is reserved for a special purpose."@en ;
  foaf:page <https://www.iana.org/assignments/special-use-domain-names/special-use-domain-names.xhtml> ;
  foaf:page rfc:6761 ;
  skos:exactMatch dbr:Special-use_domain_name .

:TopLevelDomain
  rdfs:subClassOf :Domain ;
  dcterms:description "A domain that is not a subdomain of any other."@en ;
  skos:exactMatch wd:Q14296 , dbr:Top-level_domain , dbo:TopLevelDomain .

:TopLevelDomain-CountryCode
  rdfs:subClassOf :TopLevelDomain ;
  dcterms:description "A domain name for a country."@en ;
  skos:exactMatch wd:Q42032 , dbr:Country_code_top-level_domain .

:TopLevelDomain-Generic
  rdfs:subClassOf :TopLevelDomain ;
  dcterms:description "A generic domain name."@en ;
  skos:exactMatch wd:Q29469 , dbr:Generic_top-level_domain .

:TopLevelDomain-GenericRestricted
  rdfs:subClassOf :TopLevelDomain , :TopLevelDomain-Generic ;
  dcterms:description "A generic domain name with restricted eligibility."@en .

:TopLevelDomain-Infrastructure
  rdfs:subClassOf :TopLevelDomain ;
  dcterms:description "A domain name used for internet infrastructure."@en .

:TopLevelDomain-Sponsored
  rdfs:subClassOf :TopLevelDomain , :TopLevelDomain-Generic ;
  dcterms:description "A domain name for specific communities sponsored by an organization."@en ;
  skos:exactMatch wd:Q29380 , dbr:Sponsored_top-level_domain .

:TopLevelDomain-Proposed
  rdfs:subClassOf :TopLevelDomain ;
  dcterms:description "A proposed domain name, not yet incorporated into the registry."@en ;
  skos:exactMatch wd:Q634997 , dbr:Proposed_top-level_domain .

:TopLevelDomain-Test
  rdfs:subClassOf :TopLevelDomain ;
  dcterms:description "A domain name used for testing."@en .


:address
  a owl:ObjectProperty ;
  schema:domainIncludes :Domain ;
  rdfs:range :IP ;
  dcterms:description "Links a resolved IP address to the domain."@en .

:delegationRecordPage
  a owl:ObjectProperty ;
  schema:domainIncludes :TopLevelDomain ;
  rdfs:range foaf:Document ;
  dcterms:description "Links a page describing the delegation of the top-level domain."@en .

:sponsor
  a owl:ObjectProperty ;
  schema:domainIncludes :TopLevelDomain ;
  rdfs:range foaf:Agent ;
  dcterms:description "Specifies the sponsor of the top-level domain."@en .

:subDom
  a owl:ObjectProperty ;
  rdfs:domain :Domain ;
  rdfs:range :Domain ;
  dcterms:description "Links to a subdomain of the domain."@en .

:whoIsRecord
  a owl:DatatypeProperty ;
  schema:domainIncludes :Domain ;
  schema:domainIncludes :IP ;
  rdfs:range xsd:string ;
  dcterms:description "Stores the response from a WHOIS server for the domain or IP address."@en .

:hasWhoIsServer
  a owl:ObjectProperty ;
  schema:domainIncludes :Domain ;
  schema:domainIncludes :IP ;
  schema:rangeIncludes :Domain ;
  dcterms:description "Links to the domain of the WHOIS server used for the domain or IP address."@en .

:rdapRecord
  a owl:ObjectProperty ;
  schema:domainIncludes :Domain ;
  schema:domainIncludes :IP ;
  rdfs:range rdfs:Resource ;
  dcterms:description "Links to the resource storing an RDAP record about the domain or IP address."@en .

:hasRdapServer
  a owl:ObjectProperty ;
  schema:domainIncludes :Domain ;
  schema:domainIncludes :IP ;
  schema:rangeIncludes :Domain ;
  dcterms:description "Links to the domain of the RDAP server used for the domain or IP address."@en .


:IP
  rdfs:subClassOf :Host ;
  dcterms:description "An IP address of any type."@en ;
  owl:disjointWith :Domain ;
  skos:exactMatch wd:Q11135 , dbr:IP_address .

:IPv4
  rdfs:subClassOf :IP ;
  dcterms:description "An IPv4 address."@en .

:IPv6
  rdfs:subClassOf :IP ;
  dcterms:description "An IPv6 address."@en ;
  skos:exactMatch wd:Q11097 .

:IP-Future
  rdfs:subClassOf :IP ;
  dcterms:description "A future IP address used in a URI."@en .


# Port

:Port
  dcterms:description "A port for an internet protocol, with a specific number."@en ;
  foaf:page <https://www.iana.org/assignments/service-names-port-numbers/service-names-port-numbers.xhtml> ;
  skos:exactMatch wd:Q858321 , <http://dbpedia.org/resource/Port_(computer_networking)> .


# Protocol

:Protocol
  dcterms:description "An internet protocol, such as TCP or UDP."@en ;
  foaf:page <https://www.iana.org/assignments/protocol-numbers/protocol-numbers.xhtml> ;
  foaf:age rfc:791 , rfc:8200 ;
  skos:exactMatch wd:Q15836568 , dbr:Communication_protocol .


:ProtocolDatatype
  dcterms:description "The identifier of a protocol."@en .


# Service

:Service
  dcterms:description "A named internet service, running on specific ports."@en ;
  foaf:page <https://www.iana.org/assignments/service-names-port-numbers/service-names-port-numbers.xhtml> ;
  skos:exactMatch wd:Q1640628 , dbr:Network_service .


:ServiceDatatype
  dcterms:description "The identifier of a named service."@en .


# MIME type

:Mimetype
  dcterms:description "A media type representing a format or a collection of related formats."@en ;
  foaf:page <https://www.iana.org/assignments/media-types/media-types.xhtml> ;
  foaf:page rfc:2046 ;
  skos:exactMatch wd:Q1667978 , dbr:Media_type .


:MimetypeDatatype
  dcterms:description "The identifier of a MIME type."@en .


:mimeParams
  a owl:ObjectProperty ;
  schema:domainIncludes :Mimetype ;
  rdfs:range :URIPart ;
  dcterms:description "Specifies the parameters of a MIME type."@en .


# Suffix

:Suffix
  dcterms:description "A filename extension, commonly corresponding to a format."@en ;
  skos:exactMatch wd:Q186157 , dbr:Filename_extension .


:SuffixDatatype
  dcterms:description "The identifier of a suffix, without the dot."@en .


# Format

:Format
  dcterms:description "A file format, defining the structure of a file."@en ;
  skos:exactMatch wd:Q235557 , dbr:File_format , formats:Format .


# URI field

:URIField
  rdfs:subClassOf rdf:Property ;
  dcterms:description "A field in the query or fragment portion of a URI."@en .


:URIFieldDatatype
  dcterms:description "The identifier of a URI field, percent-decoded."@en .


# URN namespace

:URNNamespace
  dcterms:description "A namespace used by a Uniform Resource Identifier."@en ;
  foaf:page <https://www.iana.org/assignments/urn-namespaces/urn-namespaces.xhtml> ;
  foaf:page rfc:8141 ;
  skos:exactMatch wd:Q69647581 .

:URNNamespace-Formal
  rdfs:subClassOf :URNNamespace ;
  dcterms:description "A URN namespace with formal registration."@en .

:URNNamespace-Informal
  rdfs:subClassOf :URNNamespace ;
  dcterms:description "A URN namespace with informal registration."@en .

:URNNamespace-Experimental
  rdfs:subClassOf :URNNamespace ;
  dcterms:description "An unregistered experimental URN namespace."@en .

:URNNamespaceDatatype
  dcterms:description "The identifier of a URN namespace."@en .


# Well-known suffix

:WellKnownURISuffix
  dcterms:description "The identifier of a well-known resource."@en ;
  foaf:page <https://www.iana.org/assignments/well-known-uris/well-known-uris.xhtml> ;
  foaf:page rfc:8615 .


:WellKnownURISuffixDatatype
  dcterms:description "The identifier of a well-known URI suffix."@en .


# URI part

:URIPart
  dcterms:description "A non-hierarchical part of a URI, either a query or a fragment."@en .

:URIPart-XPointer
  rdfs:subClassOf :URIPart;
  dcterms:description "A URI fragment in the XPointer format."@en ;
  foaf:page <https://www.w3.org/TR/xptr/> .

:URIPart-Media
  rdfs:subClassOf :URIPart ;
  dcterms:description "A URI query or fragment in the Media Fragments format."@en ;
  foaf:page <https://www.w3.org/TR/media-frags/> .


:URIPartDatatype
  dcterms:description "The query or fragment portion of a URI, undecoded."@en .

:URIPartDatatype-Decoded
  dcterms:description "The query or fragment portion of a URI, percent-decoded."@en .


# Other

dbp:mime
  schema:domainIncludes :Format ;
  schema:rangeIncludes :Mimetype ;
  skos:exactMatch formats:media_type , wdt:P1163 .


dbp:extension
  schema:domainIncludes :Format ;
  schema:rangeIncludes :Suffix ;
  skos:exactMatch formats:preferred_suffix , wdt:P1195 .


dbp:cctld
  schema:rangeIncludes :TopLevelDomain-CountryCode ;
  skos:broadMatch wdt:P78 .


dbp:extendedFrom
  schema:domainIncludes :Mimetype ;
  schema:rangeIncludes :Mimetype .


dbp:ports
  schema:domainIncludes :Service ;
  schema:rangeIncludes :Port .

skos:notation
  schema:domainIncludes
    :URIRefernce , :URIScheme , :Host , :Port , :Protocol ,
    :Service , :Mimetype , :Suffix , :URIField , :URNNamespace ,
    :WellKnownURISuffix , :URIPart ;
  schema:rangeIncludes
    xsd:anyURI , :URIDatatype-IRI , :URIDatatype-ASCII , :URISchemeDatatype , :HostDatatype , :HostDatatype-Encoded ,
    xsd:hexBinary , xsd:base64Binary , xsd:unsignedShort , :ProtocolDatatype ,
    :ServiceDatatype , :MimetypeDatatype , :SuffixDatatype , :URIFieldDatatype ,
    :URNNamespaceDatatype , :WellKnownURISuffixDatatype , :URIPartDatatype , :URIPartDatatype-Decoded .

# Deprecated

:Query
  dcterms:description "Deprecated. Both query and fragment are identified using the same class."@en .

:QueryKey
  dcterms:description "Deprecated. URI fields are treated as properties."@en .

:usedForFormat
  dcterms:description "Deprecated. Its usage was replaced by an inverse property dbp:mime."@en .

:Statement
  dcterms:description "Deprecated. Reified URI statements shall be described in another way."@en .

:object
  rdfs:domain :Statement .
:predicate
  rdfs:domain :Statement .
:subject
  rdfs:domain :Statement .

:WhoisServer
  dcterms:description "Deprecated. A WHOIS server is identified by a domain name."@en .

:Domain-Valid
  dcterms:description "Deprecated. The validity of identifiers is indicated using other means."@en .

:Domain-Invalid
  dcterms:description "Deprecated. The validity of identifiers is indicated using other means."@en .
